<div class="topSpace"></div>

Date Created: 09/03/2022 11:25:02
Tags: #Type/Proposition #Topic/Category_Theory/Later

Proved by: <i>Not Applicable</i>
References: <i>Not Applicable</i>
Justifications: <i>Not Applicable</i>

Specializations: <i>Not Applicable</i>
Generalizations: <i>Not Applicable</i>

``` ad-Proposition
title: Proposition.

Let $\cat{C}$ and $\cat{D}$ be categories and consider a covariant functor $\ms{F}:\cat{C}\to\cat{D}$. Then $\ms{F}\circ\Id_\cat{C}=\ms{F}=\Id_\cat{D}\circ\ms{F}$. In other words, the diagram

![[Images/2022-03-09_122512/image.svg|230]]

commutes.

```

<i>Proof.</i> We need to prove that
$$\begin{equation}
    \l(\ms{F}\circ\Id_\cat{C}\r)^{\Obj}=\ms{F}^{\Obj}=\l(\Id_\cat{D}\circ\ms{F}\r)^{\Obj}
\end{equation}$$
and, for all $X,Y\in\Obj\l(\cat{C}\r)$, that
$$\begin{equation}
    \begin{gathered}
        \dom\l(\ms{F}\circ\Id_\cat{C}\r)^{\Hom}=\dom\l(\ms{F}^{\Hom}\r)=\dom\l(\Id_\cat{D}\circ\ms{F}\r)^{\Hom}\\
        \cdm\l(\ms{F}\circ\Id_\cat{C}\r)^{\Hom}=\cdm\l(\ms{F}^{\Hom}\r)=\cdm\l(\Id_\cat{D}\circ\ms{F}\r)^{\Hom},\textrm{ and}\\
        \l(\ms{F}\circ\Id_\cat{C}\r)^{\Hom}=\ms{F}^{\Hom}=\l(\Id_\cat{D}\circ\ms{F}\r)^{\Hom}.
    \end{gathered}
    \cref{\ast}
\end{equation}$$
* Let $\mc{I}_\cat{C}:\Obj\l(\cat{C}\r)\to\Obj\l(\cat{C}\r)$ be the identity class function on $\cat{C}$; that is, let $\mc{I}\l(X,Y\r)$ be the formula that holds exactly when $X,Y\in\Obj\l(\cat{C}\r)$ and $X=Y$. Similarly, define $\mc{I}_\cat{D}:\cat{D}\to\cat{D}$. Take $X\in\Obj\l(\cat{C}\r)$ and observe that
$$\begin{equation}
    \begin{alignedat}{2}
        \l(\ms{F}\circ\Id_\cat{C}\r)^{\Obj}\l(X\r)&=\ms{F}^{\Obj}\l(\mc{I}_\cat{C}\l(X\r)\r)&&\textrm{Definition of composition of functors}\\
        &=\ms{F}^{\Obj}\l(X\r)&&\textrm{Definition of identity class function}\\
        &=\mc{I}_\cat{D}\l(\ms{F}^{\Obj}\l(X\r)\r)&&\ms{F}^{\Obj}\l(X\r)\in\Obj\l(\cat{D}\r)\textrm{; definition of identity functor}\\
        &=\l(\Id_\cat{D}\circ\ms{F}\r)^{\Obj}\l(X\r).\ \ \ \ \ \ \ \ &&\textrm{Definition of composition of functors}
    \end{alignedat}
    \cref{1}
\end{equation}$$
* Take $X,Y\in\Obj\l(\cat{C}\r)$ and recall that
$$\begin{equation}
    \begin{aligned}
        \ms{F}^{\Hom}:\Hom_\cat{C}\!\l(X,Y\r)&\to\Hom_\cat{D}\!\l(\ms{F}^{\Obj}\l(X\r),\ms{F}^{\Obj}\l(Y\r)\r)\\
        f&\mapsto\ms{F}^{\Hom}\l(f\r).
    \end{aligned}
\end{equation}$$
By definition, the morphism part of the composite functors are the morphisms
$$\begin{equation}
    \begin{aligned}
        \l(\ms{F}\circ\Id_\cat{C}\r)^{\Hom}:\Hom_\cat{C}\!\l(X,Y\r)&\to\Hom_\cat{D}\!\l(\l(\ms{F}\circ\Id_\cat{C}\r)^{\Obj}\l(X\r),\l(\ms{F}\circ\Id_\cat{C}\r)^{\Obj}\l(Y\r)\r)\\
        f&\mapsto\ms{F}^{\Hom}\l(\id_{\Hom_\cat{C}\l(X,Y\r)}\l(f\r)\r)
    \end{aligned}
\end{equation}$$
and
$$\begin{equation}
    \begin{aligned}
        \l(\Id_\cat{D}\circ\ms{F}\r)^{\Hom}:\Hom_\cat{C}\!\l(X,Y\r)&\to\Hom_\cat{D}\!\l(\l(\Id_\cat{D}\circ\ms{F}\r)^{\Obj}\l(X\r),\l(\Id_\cat{D}\circ\ms{F}\r)^{\Obj}\l(Y\r)\r)\\
        f&\mapsto\id_{\Hom_\cat{D}\l(X,Y\r)}\l(\ms{F}^{\Hom}\l(f\r)\r).
    \end{aligned}
\end{equation}$$
The assertions in ($\,\ast\,$) are immediately seen by simplifying and applying the results from ($\,1\,$).<span style="float:right;">$\blacksquare$</span>
